vera/VerilogToSMT.v
@@ -218,47 +218,112 @@ Equations transfer_initial (stmt : Verilog.statement) : transf (list SMTLib.term
     raise "VerilogToSMT: Invalid expression in initial block"%string
 .
 
-Equations transfer_var (name__smt : smtname) (var : Verilog.variable) : (string * smtname * width) :=
-  | name__smt, (Verilog.MkVariable vec storage name) =>
-      (name, name__smt, (Verilog.vector_declaration_width vec)).
+Equations assign_vars (start : smtname) (vars : list Verilog.variable) : list (Verilog.variable * smtname) :=
+  assign_vars start (var :: rest) :=
+    (var, start) :: (assign_vars (1 + start) rest);
+  assign_vars start nil :=
+    nil.
 
-Equations transfer_vars (start : nat) (vars : list Verilog.variable) : list (string * smtname * width) :=
-  | start, var :: rest =>
-      transfer_var start var :: (transfer_vars (1 + start) rest)
-  | start, nil => nil.
+Import VerilogSemantics.CombinationalOnly.
 
-Definition mk_var_map (vars : list (string * smtname * width)) : StrFunMap.t (smtname * width) :=
+Lemma assign_vars_vars start vars :
+  map fst (assign_vars start vars) = vars.
+Proof.
+  revert start.
+  induction vars; intros;
+    simp assign_vars in *; cbn in *.
+  - reflexivity.
+  - rewrite IHvars. reflexivity.
+Qed.
+
+Lemma assign_vars_smtname_start start vars :
+  Forall (fun n => n >= start) (map snd (assign_vars start vars)).
+Proof.
+  revert start.
+  induction vars;
+    intros; simp assign_vars in *; cbn in *;
+    constructor.
+  - lia.
+  - specialize (IHvars (S start)).
+    revert IHvars.
+    eapply Forall_impl.
+    lia.
+Qed.
+
+Lemma assign_vars_smtname_nodup start vars :
+  NoDup (map snd (assign_vars start vars)).
+Proof.
+  revert start.
+  induction vars; intros; simp assign_vars in *; cbn in *;
+    constructor.
+  - intro contra.
+    pose proof (assign_vars_smtname_start (S start) vars).
+    eapply Forall_forall in H; try eassumption.
+    lia.
+  - eapply IHvars.
+Qed.
+
+Definition mk_var_map (vars : list (Verilog.variable * smtname)) : StrFunMap.t (smtname * width) :=
   List.fold_right
-    (fun '(verilog__name, smt__name, sort) acc => StrFunMap.insert verilog__name (smt__name, sort) acc)
+    (fun '(var, smt__name) acc => StrFunMap.insert (Verilog.varName var) (smt__name, Verilog.varWidth var) acc)
     StrFunMap.empty vars.
 
-Definition mk_bijection (name_tag : TaggedName.Tag) (vars : list (string * smtname * width)) : transf VerilogSMTBijection.t :=
-  let var_pairs := map (fun '(vname, smtname, _) => (name_tag, vname, smtname)) vars in
-  nodup_left <- assert_dec (NoDup (map fst var_pairs)) "Duplicate verilog name in var_pairs"%string ;;
-  nodup_right <- assert_dec (NoDup (map snd var_pairs)) "Duplicate smt name in var_decls"%string ;;
-  ret (VerilogSMTBijection.from_pairs var_pairs nodup_left nodup_right).
+Equations mk_bijection (tag : TaggedName.Tag) (vars : list (Verilog.variable * smtname)) : transf VerilogSMTBijection.t :=
+  mk_bijection tag ((var, name__smt) :: xs) :=
+    tail_bijection <- mk_bijection tag xs ;;
+    prf1 <- assert_dec (tail_bijection (tag, Verilog.varName var) = None) ;;
+    prf2 <- assert_dec (VerilogSMTBijection.bij_inverse tail_bijection name__smt = None) ;;
+    ret (VerilogSMTBijection.insert (tag, Verilog.varName var) name__smt tail_bijection _ _);
+  mk_bijection tag [] := ret VerilogSMTBijection.empty.
+  (* mk_bijection tag ((var, name__smt) :: xs) := *)
+  (* let var_pairs := (map (fun '(var, smt__name) => ((tag, Verilog.varName var), smt__name)) vars) in *)
+  (* nodup_left <- assert_dec (NoDup (map fst var_pairs)) "Duplicate verilog name in var_pairs"%string ;; *)
+  (* nodup_right <- assert_dec (NoDup (map snd var_pairs)) "Duplicate smt name in var_decls"%string ;; *)
+  (* ret (VerilogSMTBijection.from_pairs var_pairs nodup_left nodup_right). *)
 
-Lemma mk_bijection_map_match tag var_start vmodule m :
-  mk_bijection tag (transfer_vars var_start (Verilog.modVariables vmodule)) = inr m ->
-  SMT.match_map_verilog tag m vmodule.
+Lemma mk_bijection_cons tag x xs m m':
+  mk_bijection tag (x :: xs) = inr m ->
+  mk_bijection tag xs = inr m' ->
+  m' = VerilogSMTBijection.insert (fst x) (snd x) m.
+
+Lemma mk_bijection_smt_map_match tag start v m :
+  mk_bijection tag (assign_vars start (Verilog.modVariables v)) = inr m ->
+  SMT.match_map_verilog tag m v.
 Proof.
-  intros.
-  unfold mk_bijection in H. inv H. autodestruct.
+  Opaque VerilogSMTBijection.lookup_left.
   unfold SMT.match_map_verilog.
-  unfold VerilogSMTBijection.from_pairs. simpl.
-  clear n. (* the tags are all the same *)
-  rewrite map_map in n0; simpl in n0.
-  generalize dependent (Verilog.modVariables vmodule); intros l.
-  induction l.
-  - intros; split; intros H; solve_by_inverts 2%nat.
-  - intros; split; intros H.
+  replace (variable_names (Verilog.modVariables v)) with (variable_names (map fst (assign_vars start (Verilog.modVariables v))))
+    by now rewrite assign_vars_vars.
+  remember (assign_vars start (Verilog.modVariables v)) as assignment.
+  (* epose proof (assign_vars_smtname_start _ _) as Hstart; *)
+  (*   rewrite <- Heqassignment in Hstart. *)
+  epose proof (assign_vars_smtname_nodup _ _) as Hnodup;
+    rewrite <- Heqassignment in Hnodup.
+  clear v start Heqassignment.
+  generalize dependent Hnodup.
+  generalize dependent m.
+  induction assignment; intros * ? Hbijection.
+  - unfold mk_bijection in Hbijection; inv Hbijection; autodestruct.
+    split; intros H; cbn in *; solve_by_inverts 2%nat.
+  - unfold variable_names.
+    unfold mk_bijection in Hbijection; inv Hbijection; autodestruct.
+    intros.
+    split; intros H.
     + destruct H as [smtName H].
-      simp transfer_vars in *.
-      rewrite List.map_cons in H.
-      rewrite VerilogSMTBijection.lookup_left_some_iff in H.
-      admit.
-    + admit.
-Admitted.
+      erewrite VerilogSMTBijection.from_pairs_cons in H.
+      cbn in H.
+      destruct
+        (dec_eq_string verilogName (Verilog.varName v)),
+        (TaggedName.dec_eq_tag tag tag);
+        cbn in H; cbn;
+        try contradiction.
+      * eauto.
+      * right. unfold variable_names in IHassignment.
+        eapply IHassignment.
+        -- now inv Hnodup.
+        --
+
+    rewrite map_map, map_cons.
 
 Equations verilog_to_smt (name_tag : TaggedName.Tag) (var_start : nat) (vmodule : Verilog.vmodule)
   : transf SMT.smt_with_namemap :=
